Refactor EveryPrepareClientOpMatchesRecordedPrePrepare predicate.
We refactor the predicate, which is part of the Inv to not bind the
state of the network to the internal state of the replicas.
Added reasoning in the case analysis for preserving
EveryCommitIsSupportedByPreviouslySentPrepares.

docs/sbft-formal-model/proof.dfy
@@ -216,17 +216,34 @@ module Proof {
              && commitMsg.payload.operationWrapper == recordedPrePrepare.value.payload.operationWrapper)
   }
 
-  predicate {:opaque} EveryPrepareClientOpMatchesRecordedPrePrepare(c:Constants, v:Variables) {
+  predicate {:opaque} EveryPrepareClientOpMatchesRecordedPrePrepare_deprecated(c:Constants, v:Variables) {
     && v.WF(c)
-    && (forall prepareMsg | && prepareMsg in v.network.sentMsgs
-                           && prepareMsg.payload.Prepare?
-                           && IsHonestReplica(c, prepareMsg.sender)
-                           && var replicaVariables := v.hosts[prepareMsg.sender].replicaVariables;
-                           && var replicaConstants := c.hosts[prepareMsg.sender].replicaConstants;
-                           && prepareMsg.payload.seqID in replicaVariables.workingWindow.getActiveSequenceIDs(replicaConstants)
-                           && prepareMsg.payload.view == replicaVariables.view
+    && (forall prepareMsg | 
+                      && prepareMsg in v.network.sentMsgs
+                      && prepareMsg.payload.Prepare?
+                      && IsHonestReplica(c, prepareMsg.sender)
+                      && var replicaVariables := v.hosts[prepareMsg.sender].replicaVariables;
+                      && var replicaConstants := c.hosts[prepareMsg.sender].replicaConstants;
+                      && prepareMsg.payload.seqID in replicaVariables.workingWindow.getActiveSequenceIDs(replicaConstants)
+                      && prepareMsg.payload.view == replicaVariables.view
           :: && var recordedPrePrepare := 
                 v.hosts[prepareMsg.sender].replicaVariables.workingWindow.prePreparesRcvd[prepareMsg.payload.seqID];
+             && recordedPrePrepare.Some?
+             && prepareMsg.payload.operationWrapper == recordedPrePrepare.value.payload.operationWrapper)
+  }
+
+  predicate {:opaque} EveryPrepareClientOpMatchesRecordedPrePrepare(c:Constants, v:Variables) {
+    && v.WF(c)
+    && (forall prepareMsg:Network.Message<Messages.Message> | 
+          && prepareMsg.payload.Prepare?
+          && IsHonestReplica(c, prepareMsg.sender)
+          && var replicaVariables := v.hosts[prepareMsg.sender].replicaVariables;
+          && var replicaConstants := c.hosts[prepareMsg.sender].replicaConstants;
+          && prepareMsg.sender in replicaVariables.workingWindow.preparesRcvd[prepareMsg.payload.seqID].Keys
+          && replicaVariables.workingWindow.preparesRcvd[prepareMsg.payload.seqID][prepareMsg.sender] == prepareMsg
+          //&& prepareMsg.payload.seqID in replicaVariables.workingWindow.getActiveSequenceIDs(replicaConstants)
+          //&& prepareMsg.payload.view == replicaVariables.view
+          :: && var recordedPrePrepare := v.hosts[prepareMsg.sender].replicaVariables.workingWindow.prePreparesRcvd[prepareMsg.payload.seqID];
              && recordedPrePrepare.Some?
              && prepareMsg.payload.operationWrapper == recordedPrePrepare.value.payload.operationWrapper)
   }
@@ -623,6 +640,19 @@ module Proof {
     }
   }
 
+  lemma CountPrepareMessages(proofSet:Replica.PrepareProofSet)
+    requires forall sender | sender in proofSet.Keys :: proofSet[sender].sender == sender
+    ensures |proofSet.Values| == |proofSet.Keys|
+  {
+    if |proofSet.Keys| > 0 {
+      var element :| element in proofSet.Keys;
+      var subMap := MapRemoveOne(proofSet, element);
+      CountPrepareMessages(subMap);
+      assert proofSet.Values == subMap.Values + {proofSet[element]};
+      assert proofSet.Keys == subMap.Keys + {element};
+    }
+  }
+
   lemma HonestPreservesEveryCommitIsSupportedByPreviouslySentPrepares(c: Constants, v:Variables, v':Variables, step:Step, h_v:Replica.Variables, h_step:Replica.Step)
     requires Inv(c, v)
     requires HonestReplicaStepTaken(c, v, v', step, h_v, h_step)
@@ -643,8 +673,23 @@ module Proof {
                 reveal_RecordedPreparesMatchHostView();
                 reveal_EveryPrepareClientOpMatchesRecordedPrePrepare();
                 reveal_RecordedPreparesInAllHostsRecvdCameFromNetwork();
-                var recordedPrepares := set | msg in h_v.workingWindow.preparesRcvd[commitMsg.payload.seqID];
-                assert x <= sentPreparesForSeqID(c, v, commitMsg.payload.view, commitMsg.payload.seqID, commitMsg.payload.operationWrapper);
+                var recordedPrepares := h_v.workingWindow.preparesRcvd[commitMsg.payload.seqID].Values;
+                CountPrepareMessages(h_v.workingWindow.preparesRcvd[commitMsg.payload.seqID]);
+                var sentPrepares := sentPreparesForSeqID(c, v, commitMsg.payload.view, commitMsg.payload.seqID, commitMsg.payload.operationWrapper);
+                assert recordedPrepares <= sentPrepares by {
+                  forall msg | msg in recordedPrepares ensures msg in sentPrepares {
+                        assert msg in v.network.sentMsgs;
+                        assert msg.payload.Prepare?;
+                        assert msg.payload.view == commitMsg.payload.view;
+                        assert msg.payload.seqID == commitMsg.payload.seqID;
+                        assert msg in v.network.sentMsgs;
+                        assert msg.payload.operationWrapper == h_v.workingWindow.prePreparesRcvd[commitMsg.payload.seqID].value.payload.operationWrapper;
+                        assert msg.payload.operationWrapper == commitMsg.payload.operationWrapper;
+                        assert msg.sender in getAllReplicas(c);
+                  }
+                }
+                Library.SubsetCardinality(recordedPrepares, sentPrepares);
+                // assert x <= sentPreparesForSeqID(c, v, commitMsg.payload.view, commitMsg.payload.seqID, commitMsg.payload.operationWrapper);
                 assert QuorumOfPreparesInNetwork(c, v, commitMsg.payload.view, 
                         commitMsg.payload.seqID, commitMsg.payload.operationWrapper);
                 assert QuorumOfPreparesInNetwork(c, v', commitMsg.payload.view, 
